src/SimulationUtils.v
@@ -12,7 +12,7 @@ Require Import Arith.
    If A = B and C = D, we call it "preservation".
 
    Genarally,
-   - The Le relations is between states (S <= S'), or pairs of value and state ((v, S) <= (v', S')).
+   - The Leq relations is between states (S <= S'), or pairs of value and state ((v, S) <= (v', S')).
    - The Red relations are among the following ones:
      - Evaluation of operands.
      - Evalutaion of rvalues.
@@ -20,9 +20,9 @@ Require Import Arith.
      - Evaluation of statements.
  *)
 Definition forward_simulation {A B C D : Type}
-  (LeBA : B -> A -> Prop) (LeDC : D -> C -> Prop)
+  (LeqBA : B -> A -> Prop) (LeqDC : D -> C -> Prop)
   (RedAC : A -> C -> Prop) (RedBD : B -> D -> Prop) :=
-  forall a c, RedAC a c -> forall b, LeBA b a -> exists d, LeDC d c /\ RedBD b d.
+  forall a c, RedAC a c -> forall b, LeqBA b a -> exists d, LeqDC d c /\ RedBD b d.
 
 (* The reflexive-transitive R* closure of a relation R. *)
 Inductive refl_trans_closure {A : Type} (R : A -> A -> Prop) : A -> A -> Prop :=
@@ -64,12 +64,12 @@ Qed.
 (* Generally, to prove preservation when the relation is a reflexive transitive closure, it
  * suffices to prove it for the base cases. *)
 Lemma preservation_by_base_case {A B : Type}
-  (LeA : A -> A -> Prop) (LeB : B -> B -> Prop) (RedAB : A -> B -> Prop) :
-  forward_simulation LeA (refl_trans_closure LeB) RedAB RedAB ->
-  forward_simulation (refl_trans_closure LeA) (refl_trans_closure LeB) RedAB RedAB.
+  (LeqA : A -> A -> Prop) (LeqB : B -> B -> Prop) (RedAB : A -> B -> Prop) :
+  forward_simulation LeqA (refl_trans_closure LeqB) RedAB RedAB ->
+  forward_simulation (refl_trans_closure LeqA) (refl_trans_closure LeqB) RedAB RedAB.
 Proof.
-  intros H a b red_ab a' Le_a_a'. revert b red_ab.
-  induction Le_a_a' as [ | | a2 a1 a0 _ IH0 _ IH1].
+  intros H a b red_ab a' Leq_a_a'. revert b red_ab.
+  induction Leq_a_a' as [ | | a2 a1 a0 _ IH0 _ IH1].
   - intros. eapply H; eassumption.
   - intros. eexists. split; [reflexivity | eassumption].
   - intros b0 Red_a0_b0.
@@ -82,7 +82,7 @@ Qed.
    - there exists d0 such that c -> d0
    - there exists d1 such that b <= d1
    - d0 = d1
-   This lemma allows us to not exhibit the terms d0 and d1 explicitely. As the relations LeCD and
+   This lemma allows us to not exhibit the terms d0 and d1 explicitely. As the relations LeqCD and
    RedBD are generally inductively defined, these terms are constructed by applying inductive
    constructors. This is why the constructors of the relation should be on the form:
    - red S E[S] for the reduction
@@ -91,17 +91,17 @@ Qed.
    states_eq.
  *)
 Lemma complete_square_diagram {B C D : Type}
-  (LeDC : D -> C -> Prop) (RedBD : B -> D -> Prop) b c (d0 d1 : D) :
-  LeDC d0 c -> RedBD b d1 -> d0 = d1
-  -> exists d, LeDC d c /\ RedBD b d.
+  (LeqDC : D -> C -> Prop) (RedBD : B -> D -> Prop) b c (d0 d1 : D) :
+  LeqDC d0 c -> RedBD b d1 -> d0 = d1
+  -> exists d, LeqDC d c /\ RedBD b d.
 Proof. intros ? ? <-. exists d0. auto. Qed.
 
-(* Generally, two types A and B will have a canonical relation Le. *)
-Class Le (A B : Type) :=
-{ le : A -> B -> Prop }.
+(* Generally, two types A and B will have a canonical relation Leq. *)
+Class Leq (A : Type) :=
+{ leq : A -> A -> Prop }.
 
-Definition preservation {A B} `{LeA : Le A A} `{LeB : Le B B} (RedAB : A -> B -> Prop) :=
-  forward_simulation (@le A A LeA) (@le B B LeB) RedAB RedAB.
+Definition preservation {A B} `{LeqA : Leq A} `{LeqB : Leq B} (RedAB : A -> B -> Prop) :=
+  forward_simulation (@leq A LeqA) (@leq B LeqB) RedAB RedAB.
 
 (* Relations are generally defined for types of states, for any semantics between LLBC# and
    HLPL. In the following section, we will define the relation S <= S' for states,
@@ -109,34 +109,34 @@ Definition preservation {A B} `{LeA : Le A A} `{LeB : Le B B} (RedAB : A -> B ->
    We also specify a well-formedness predicate for states. Indeed, some preservation properties
    require the well-formedness to be proven.
 *)
-Class LeBase state := {
-  le_base : state -> state -> Prop;
+Class LeqBase state := {
+  leq_base : state -> state -> Prop;
   well_formed : state ->  Prop;
-  le_base_preserves_well_formedness Sl Sr : well_formed Sr -> le_base Sl Sr -> well_formed Sl;
+  leq_base_preserves_well_formedness Sl Sr : well_formed Sr -> leq_base Sl Sr -> well_formed Sl;
 }.
 
-Global Instance LeState state `(LeBase state) : Le (state) (state) :=
-{ le := refl_trans_closure le_base }.
+Global Instance LeqState state `(LeqBase state) : Leq state :=
+{ leq := refl_trans_closure leq_base }.
 
-Section LeValStateUtils.
+Section LeqValStateUtils.
   Context `{State state V}.
-  Context `{LB : LeBase state}.
+  Context `{LB : LeqBase state}.
 
-  Definition le_val_state_base (vSl vSr : V * state) :=
+  Definition leq_val_state_base (vSl vSr : V * state) :=
     forall a, fresh_anon (snd vSl) a -> fresh_anon (snd vSr) a ->
-    le_base ((snd vSl),, a |-> fst vSl) ((snd vSr),, a |-> fst vSr).
+    leq_base ((snd vSl),, a |-> fst vSl) ((snd vSr),, a |-> fst vSr).
 
   (* For pair of value and states, we have:
      (v, S) <= (v', S') ::= S,, _ |-> v <= S', _ |-> v'
    *)
-  Global Instance LeStateVal : Le (V * state) (V * state) :=
-  { le := refl_trans_closure le_val_state_base }.
+  Global Instance LeqStateVal : Leq (V * state) :=
+  { leq := refl_trans_closure leq_val_state_base }.
 
-  Lemma prove_le_val_state vSl vm Sm vr Sr
+  Lemma prove_leq_val_state vSl vm Sm vr Sr
     (G : forall a, fresh_anon Sm a -> fresh_anon Sr a ->
-         exists vSm, le_base vSm Sr,, a |-> vr /\ vSm = Sm,, a |-> vm) :
-    @le _ _ LeStateVal vSl (vm, Sm) ->
-    @le _ _ LeStateVal vSl (vr, Sr).
+         exists vSm, leq_base vSm Sr,, a |-> vr /\ vSm = Sm,, a |-> vm) :
+    @leq _ LeqStateVal vSl (vm, Sm) ->
+    @leq _ LeqStateVal vSl (vr, Sr).
   Proof.
     intros ?. etransitivity; [eassumption | ]. constructor.
     intros a ? ?. cbn in *. destruct (G a) as (? & ? & ->); [assumption.. | ]. assumption.
@@ -147,17 +147,17 @@ Section LeValStateUtils.
      closure.
      We're going to give similar statements, but these types, the hypothesis uses the relation le.
    *)
-  Lemma preservation_by_base_case_le_state_le_val_state
+  Lemma preservation_by_base_case_leq_state_leq_val_state
     (red : state -> (V * state) -> Prop) :
-    forward_simulation (@le_base _ LB) (@le _ _ LeStateVal) red red
-    -> @preservation _ _ (@LeState _ LB) LeStateVal red.
+    forward_simulation (@leq_base _ LB) (@leq _ LeqStateVal) red red
+    -> @preservation _ _ (@LeqState _ LB) LeqStateVal red.
   Proof. apply preservation_by_base_case. Qed.
-End LeValStateUtils.
+End LeqValStateUtils.
 
-(* When proving a goal `le ?vSl (vr, Sr)`, using this tactic create three subgoals:
-   1. le_base ?vSm (Sr,, a |-> v)r
+(* When proving a goal `leq ?vSl (vr, Sr)`, using this tactic create three subgoals:
+   1. leq_base ?vSm (Sr,, a |-> v)r
    2. ?vSm = ?Sm,, a |-> ?vm
-   3. le ?vSl (?vm, ?Sm)
+   3. leq ?vSl (?vm, ?Sm)
 
    The first goal is used by applying the adequate base rule. Here, a is a fresh anon.
    The second goal is proved by rewriting (with `autorewrite with spath`) then reflexivity.
@@ -166,24 +166,24 @@ End LeValStateUtils.
    With this strategy, the states and values ?vSl, ?vSm, ?vm and ?Sm never have to be instantiated
    explicitely.
  *)
-Ltac le_val_state_step :=
+Ltac leq_val_state_step :=
   let a := fresh "a" in
-  eapply prove_le_val_state; [intros a ? ?; eexists; split | ].
+  eapply prove_leq_val_state; [intros a ? ?; eexists; split | ].
 
 Section WellFormedSimulations.
-  Context `{LB : LeBase state}.
+  Context `{LB : LeqBase state}.
   Definition well_formed_forward_simulation {B C D : Type}
-    (LeBA : B -> state -> Prop) (LeDC : D -> C -> Prop)
+    (LeqBA : B -> state -> Prop) (LeqDC : D -> C -> Prop)
     (RedAC : state -> C -> Prop) (RedBD : B -> D -> Prop) :=
-    forall a c, well_formed a -> RedAC a c -> forall b, LeBA b a -> exists d, LeDC d c /\ RedBD b d.
+    forall a c, well_formed a -> RedAC a c -> forall b, LeqBA b a -> exists d, LeqDC d c /\ RedBD b d.
 
   Definition well_formed_preservation (Red : state -> state -> Prop) :=
-    well_formed_forward_simulation (@le _ _ (@LeState _ LB)) (@le _ _ (@LeState _ LB)) Red Red.
+    well_formed_forward_simulation (@leq _ (@LeqState _ LB)) (@leq _ (@LeqState _ LB)) Red Red.
 
-  Lemma le_preserves_well_formedness Sl Sr : well_formed Sr -> le Sl Sr -> well_formed Sl.
-  Proof. intros ? H. induction H; eauto using le_base_preserves_well_formedness. Qed.
+  Lemma leq_preserves_well_formedness Sl Sr : well_formed Sr -> leq Sl Sr -> well_formed Sl.
+  Proof. intros ? H. induction H; eauto using leq_base_preserves_well_formedness. Qed.
 
-  (* Reorganizations and le are defined as reflexive-transitive closure of relations (that we are
+  (* Reorganizations and leq are defined as reflexive-transitive closure of relations (that we are
    * going to denote < and reorg). When we want to prove the preservation, ie:
 
       Sl <*  Sr
@@ -211,10 +211,10 @@ Section WellFormedSimulations.
   (* Note: for the moment, we just use natural measures. *)
   Lemma preservation_reorg (reorg : state -> state -> Prop)
     (measure : state -> nat)
-    (le_decreasing : forall a b, le_base a b -> measure a < measure b)
+    (leq_decreasing : forall a b, leq_base a b -> measure a < measure b)
     (reorg_decreasing : forall a b, reorg a b -> measure b < measure a)
     (reorg_preserves_wf : forall a b, reorg a b -> @well_formed _ LB a -> @well_formed _ LB b)
-    (H : well_formed_forward_simulation (@le_base _ LB) (@le _ _ (@LeState _ LB)) reorg (refl_trans_closure reorg)) :
+    (H : well_formed_forward_simulation (@leq_base _ LB) (@leq _ (@LeqState _ LB)) reorg (refl_trans_closure reorg)) :
     well_formed_preservation (refl_trans_closure reorg).
   Proof.
     assert (forall S S', refl_trans_closure reorg S S' -> measure S' <= measure S).
@@ -225,20 +225,20 @@ Section WellFormedSimulations.
     intros Sr -> Sr' well_formed_Sr reorg_Sr_Sr'.
     destruct reorg_Sr_Sr' as [ | Sr Sr' Sr'' reorg_Sr_Sr' ? _] using refl_trans_closure_ind_left.
     { intros. eexists. split; [eassumption | reflexivity]. }
-    intros Sl le_Sl_Sr.
-    destruct le_Sl_Sr as [ | Sl Sm Sr ? _ le_Sm_Sr] using refl_trans_closure_ind_right.
+    intros Sl leq_Sl_Sr.
+    destruct leq_Sl_Sr as [ | Sl Sm Sr ? _ leq_Sm_Sr] using refl_trans_closure_ind_right.
     { eexists. split; [reflexivity | ]. transitivity Sr'; [constructor | ]; assumption. }
-    specialize (H _ _ well_formed_Sr reorg_Sr_Sr' _ le_Sm_Sr). destruct H as (Sm' & le_Sm'_Sr' & reorg_Sm_Sm').
-    assert (exists Sl', le Sl' Sm' /\ refl_trans_closure reorg Sl Sl')
+    specialize (H _ _ well_formed_Sr reorg_Sr_Sr' _ leq_Sm_Sr). destruct H as (Sm' & leq_Sm'_Sr' & reorg_Sm_Sm').
+    assert (exists Sl', leq Sl' Sm' /\ refl_trans_closure reorg Sl Sl')
       as (Sl' & ? & ?)
-    by eauto using le_base_preserves_well_formedness.
-    assert (exists Sm'', le Sm'' Sr'' /\ refl_trans_closure reorg Sm' Sm'')
+    by eauto using leq_base_preserves_well_formedness.
+    assert (exists Sm'', leq Sm'' Sr'' /\ refl_trans_closure reorg Sm' Sm'')
       as (Sm'' & ? & ?)
       by eauto.
-    assert (exists Sl'', le Sl'' Sm'' /\ refl_trans_closure reorg Sl' Sl'')
+    assert (exists Sl'', leq Sl'' Sm'' /\ refl_trans_closure reorg Sl' Sl'')
       as (? & ? & ?).
     { eapply IH; [ | reflexivity | | eassumption..];
-      eauto using Nat.le_lt_trans, le_preserves_well_formedness. }
+      eauto using Nat.le_lt_trans, leq_preserves_well_formedness. }
     eexists. split; [transitivity Sm'' | transitivity Sl']; eassumption.
   Qed.
 End WellFormedSimulations.
